<section xml:id="Tut1Afr">
  <title>W214 LineÃªre Algebra 2019, Tutoriaal 1</title>
  <shorttitle>Tutoriaal 1</shorttitle>
  <introduction>
  	<p>
  		Tutorial 1 bevat <xref ref="ACh1Sec1Intro"/> tot en met die einde van <xref ref="ACh1Sec5ResultsVectorSpace"/>. Die volgende oefeninge is gekies.
  	</p>
  </introduction>


  <exercises>
    <exercise>
      <statement>
        <p>
          Prove that set <m>C</m> from <xref ref="ACh1Sec1Intro">Section</xref>
          together with the addition operation <xref ref="add_in_C"/>,
          the zero vector <xref ref="zero_in_C" /> and the scalar multiplication operation <xref ref="sm_in_C" /> forms a vector space.
        </p>
      </statement>
      <solution>
      <p>
      Firstly, we note that the addition operator, the zero vector, and scalar multiplication are all well-defined. We are required to check R1-R8.
      </p>
      <p>
        
          <p>
           R1: Let
            <md>
            <mrow>p = a_4 x^4 + a_3 x^3 + a_2 x^2 + a_1 x + a _0 </mrow>
            <mrow>q = b_4 x^4 + b_3 x^3 + b_2 x^2 + b_1 x + b _0. </mrow>
            </md>
      Then <md>
      <mrow>p + q \amp = (a_4 +b_4)x^4 + \ldots + (a_0 +b_0) \amp \mbox{(defn of addition in C)}</mrow>
      <mrow> \amp = (b_4 + a_4)x^4 + \ldots (b_0 + a_0) \amp \mbox{(s+t = t+s for real  numbers s,t)}</mrow>
      <mrow> \amp = q +p \amp \mbox{(defn of addition in C)} </mrow>
           </md>
            </p>


      <p>
        R2:
        Let <m> r = c_4 x^4 + \ldots c_0 </m>
         Then
         <md>
         <mrow> (p+q) +r \amp = \left[a_4 +b_4)x^4 + \ldots + (a_0 +b_0)\right] + (c_4 x^4 + \ldots c_0) \amp \mbox{(defn of addition in C)} </mrow>
         <mrow> \amp =  ((a_4 +b_4) + c_4)x^4 + \ldots + ((a_0 +b_0) + c_4) \amp \mbox{(defn of addition in C)}</mrow>
         <mrow> \amp = (a_4 +(b_4 + c_4)x^4 + \ldots + (a_0 +(b_0 + c_4)) \amp \mbox{((s+t)+u = s +(t+u) for real numbers s,t,u)}</mrow>
      <mrow> \amp = \left[ (a_4 x^4 + \ldots a_0 \right] + \left[(b_4+c_4) x^4 + \ldots (b_0 + c_0) \right]  \amp \mbox{(defn of addition in C)}</mrow>
      <mrow> \amp = p + (q +r)  \amp \mbox{(defn of addition in C)}</mrow>
       </md>
      </p>

      <p>
      R3: Let <m> z = 0x^4 \ldots 0 </m>.
      R3a: <md>
      <mrow> z + p \amp = (0x^4 \ldots 0) + (a_4 x^4 + \ldots a_0) \amp \mbox{(defn of addition in C)}</mrow>
      <mrow> \amp = (0 + a_4) x^4 + \ldots (0 + a_0) \amp \mbox{(defn of addition in C)} </mrow>
      <mrow> \amp = a_4 x^4 + \ldots a_0 \amp \mbox{(0 + t = t for real numbers t)}</mrow>
      <mrow> \amp = p</mrow>
      </md>
      </p>
      The rest of the rules are similar.
      </p>
      </solution>
    </exercise>

    <exercise>
      <statement>
        <p>
          Define the set <m>C^\prime</m> consisting of all polynomials of degree <em>exactly </em> 4. Show that if <m>C^\prime</m> is given the addition operation <xref ref="add_in_C"/>, the zero vector <xref ref="zero_in_C" /> and the scalar multiplication operation <xref ref="sm_in_C" /> then <m>C^\prime</m> <em> does not </em> form a vector space.
        </p>
      </statement>
      <hint>
        <p>
          Give a counterexample!
        </p>
      </hint>

      <solution>
        <p>
        We shall show that <m>C^\prime</m> is not closed under addition. 
        Let <md>
        <mrow> p \amp = x^4 </mrow>
        <mrow> q \amp = -x^4 + x^3. </mrow>
        </md>
        Then 
        <me>
        p + q = x^3.
        </me>
        But <m> x^3 </m> is not in <m> C^\prime </m>. Hence <m> C^\prime </m> is not closed under addition and so cannot be a vector space.
        </p>
      </solution>
    </exercise>

    <exercise>
      <statement>
      <p>Consider the set
        <me>
        X := \{(a_1, a_2) \in \mathbb{R}^2 : a_1 \geq 0, a_2 \geq 0\}
      </me>
      equipped with the same addition operation <xref ref="add_in_A" />,
          zero vector <xref ref="zero_in_A" /> and scalar multiplication operation <xref ref="sm_in_A"/> as in <m>A</m>. Does <m>X</m> form a vector space? If not, why not?
        </p>
      </statement>
      <solution>
        <p> <m> X </m> is not a vector space since scalar multiplication is not defined! For example, consider <m> (1,1)</m>. <m> (1,1) \in X</m> but <m> (-1)\smul (1,1) = (-1,-1)</m> is not.
        </p>
      </solution>
    </exercise>



    <exercise>
      <statement>
        <p>
          Notation quiz!
          Say whether the following combination of symbols represents a real number or a function.

          <ol>
            <li>
              <p>
                <m>f</m>
              </p>
            </li>

            <li>
              <p>
                <m>f(x)</m>
              </p>
            </li>

            <li>
              <p>
                <m>k \smul f</m>
              </p>
            </li>

            <li>
              <p>
                <m>(k \smul f)(x)</m>
              </p>
            </li>
          </ol>
        </p>
      </statement>
      <solution>
      <p>
        <ol>
          <li>
            Function
          </li>
          <li>
            Real Number
          </li>
          <li>
            Function
          </li>
          <li>
            Real Number
          </li>
        </ol>
      </p>
      </solution>
    </exercise>

    <exercise>
      <statement>
        <p>
          Let <m>X = \{a, b, c\}</m>.

          <ol>
            <li xml:id="three_functions_a">
              <p>
                Write down three different functions <m>f, g, h</m> in <m>\Fun(X)</m>.
              </p>
            </li>

            <li>
              <p>
                For each of the functions you wrote down in  <xref ref="three_functions_a"/>,
                calculate (i) <m>f + g</m> and (ii) <m>3 \smul h</m>.
              </p>
            </li>
          </ol>
        </p>
      </statement>
      <solution>
        <p>
        <ol>
          <li> 
            <md>
            <mrow> f(a)= 4 </mrow>
            <mrow> f(b) = 0 </mrow>
            <mrow> f(c) = 2 </mrow>     
            <mrow></mrow>
            <mrow> g(a)= 1 </mrow>
            <mrow> g(b) = 1 </mrow>
            <mrow> g(c) = 1 </mrow>
            <mrow></mrow>
            <mrow> h(a)= 0 </mrow>
            <mrow> h(b) = 3</mrow>
            <mrow> h(c) = 0 </mrow>
          </md>
          </li>
          <li>
          <md>
          <mrow> (f+g)(a) =5</mrow>
          <mrow> (f+g)(b) =1 </mrow>
          <mrow> (f+g)(c) = 3</mrow>
          <mrow></mrow>
          <mrow>( 3 \smul h)(a) = 0 </mrow>
          <mrow>( 3 \smul h)(b) = 9 </mrow>
          <mrow>( 3 \smul h)(c) = 0 </mrow>
          </md>
          </li>
        </ol>
        </p>
      </solution>
    </exercise>

    <exercise xml:id="strange_addition_R_2">
      <statement>
        <p>
          Define a strange new addition operation <m>\hat{+}</m> on <m>\mathbb{R}</m> by
          <me>
            x \hat{+} y := x - y, \qquad x, y \in \mathbb{R}
          </me>.
        </p>

        <p>
          Does <m>\hat{+}</m> satisfy R2?
          If it does, prove it.
          If it does not, give a counterexample.
        </p>
      </statement>
      <solution>
        <p>
          No, for example:
          <me> (1 \hat{+} 2) \hat{+} 3 = (1-2)-3 = -4</me>.
          But
          <me> 1 \hat{+} (2 \hat{+}3) = 1 - (2-3) = 2</me>.
        </p>
      </solution>
    </exercise>


    <exercise>
      <statement>
        <p>
          Construct an operation <m>\boxplus</m> on <m>\mathbb{R}</m> satisfying R1 but not R2.
        </p>
      </statement>
      <hint> 
        <p>
          Try adjusting the formula from <xref ref="strange_addition_R_2"/>.
        </p>
      </hint>
      <solution>
      <p>
        Define <m> x\boxplus y = | x - y | </m>. R1 is satisfied since <m> x \boxplus y = | x - y | = | y -x | = y \boxplus x</m>. However, R2 is not satisfied since
        <m> (1 \boxplus 2) \boxplus 3 = | |1-2| -3| = 2  </m> but <m> 1 \boxplus ( 2 \boxplus 3) = | 1 - |2-3| = 0 </m>
      </p>
      </solution>
    </exercise>

    <exercise>
      <statement>
        <p>
          Prove that for all vectors <m>\ve{v}</m> in a vector space,
          <m>-(-\ve{v}) = \ve{v}</m>.
        </p>
      </statement>
      <solution>
        <p>
          The proof is as follows:
          <md>
            <mrow>-(-v) \amp = (-1)\smul\left( (-1) \smul v\right) \amp \mbox{(defn of -v applied twice)}</mrow>
            <mrow> \amp = \left((-1)(-1)\right) \smul v \amp \mbox{(R6)}</mrow>
            <mrow> \amp = 1 \smul v </mrow>
            <mrow> \amp = v \amp \mbox{(R7)}</mrow>
          </md>
        </p>
      </solution>
    </exercise>

    <exercise>
      <statement>
      <p>
        Let <m>V</m> be a vector space. Suppose that a vector <m>\ve{v} \in V</m> satisfies
        <men>
          5\smul \ve{v} = 2 \smul \ve{v}.
        </men>
        Prove that <m>\ve{v}=\ve{0}</m>.
      </p>
      </statement>
      <solution>
        <p>
          <md>
            <mrow>\amp  5 \smul v = 2\smul v </mrow>
          <mrow> \amp \implies 5.v + (-2).v = 2.v + (-2).v </mrow>
          <mrow>\amp \implies (5 - 2).v = (2 - 2).v </mrow>
          <mrow> \amp \implies 3.v = 0.v </mrow>
          <mrow> \amp \implies (\frac{1}{3} 3).v = (\frac{1}{3} 0) v </mrow>
          <mrow> \amp \implies 1v = 0v </mrow>
          <mrow> \amp \implies v = 0</mrow>
        </md>
        </p>
      </solution>
    </exercise>

    <exercise>
      <statement>
      <p>
        If <m>k \smul \ve{v} = \ve{0}</m> in a vector space, then it necessarily follows that <m>k=0</m>.
      </p>
      </statement>
      <solution>
      <p>
        False. Take <m>\mathbb{R}^2</m> as an example. If <m>v = (0,0)</m> then
        <m>2.(0,0) = (0,0) </m> but, of course, <m> 2 \neq 0</m>.
      </p>
      </solution>
    </exercise>

    <exercise>
      <statement>
      <p>
        The empty set can be equipped with data <xref ref="D1">D1</xref>, <xref ref="D2">D2</xref>, <xref ref="D3">D3</xref> satisfying the rules of a vector space.
      </p>
    </statement>
    <solution>
    <p>
      False. In order for the empty set to be a vector space, it must have a zero vector. That is, we must be able to find some <m> v \in \text{the empty set} </m> satisfying the axioms for the zero vector. However, since the empty set has no elements in it, by definition, we cannot ever hope to find such a <m> v </m>. Hence the empty set can never be a vector space.
    </p>
    </solution>
    </exercise>

    <exercise>
      <statement>
      <p>
      Rule <xref ref="R7">R7</xref> of a vector space follows automatically from the other rules.
      </p>
      </statement>
      <solution>
      <p>
        False. Let <m>V</m> be a non-zero vector space (such as <m>\mathbb{R}^2</m>). Redefine scalar multiplication as follows
        <me> 
            k.v := 0 \mbox{ for all scalars k and all vectors v}.
        </me>
        Then <m>V</m> will satisfy all the rules of a vector space except R7. Thus it is not the case that R7 follows from the other rules.
      </p>
      </solution>
    </exercise>
</exercises>
</section>