

<appendix xmlns:xi="http://www.w3.org/2001/XInclude"  xml:id="AppBHypersurfaces">
  <title>Hypersurfaces</title>
  <definition>
    <statement>
      <p>
        Let <m>f : \mathbb{R}^{n+1} \rightarrow \mathbb{R}</m> be a function.
        The <term>zero set</term> of <m>f</m> is the subset <m>M \subset \mathbb{R}^{n+1}</m> given by
        <me>
          M := \{ \ve{x} \in \mathbb{R}^{n+1} : f(\ve{x}) = 0 \}
        </me>.
      </p>
    </statement>
  </definition>

  <definition>
    <statement>
      <p>
        We say that a subset
        <m>M \subset \mathbb{R}^{n+1}</m> is an
        <term><m>n</m>-dimensional hypersurface</term>
        if there exists a function
        <m>f : \mathbb{R}^{n+1} \rightarrow \mathbb{R}</m>
        such that <m>M</m> is the zero set of <m>f</m>,
        and if for all <m>\ve{p} \in M</m>,
        <me>
          \nabla_{\ve{p}} f \text{ exists and is not equal to }  \ve{0}
        </me>.
      </p>
    </statement>
  </definition>

  <example xml:id="hyperbola_example">
    <title>Hyperbola</title>
    <statement>
      <p>
        Let <m>f : \mathbb{R}^2 \rightarrow \mathbb{R}</m> be the function
        <me>
          f(x,y) = y^2 - x^2 - 1
        </me>
      </p>

      <p>
        Draw a picture of the zero set <m>M</m> of <m>f</m>,
        and show that it is a hypersurface.
      </p>
    </statement>
    <solution>
      <p>
        The zero level set of <m>f</m> is
        <me>
          M = \{ (x,y) \in \mathbb{R}^2 : y^2 - x^2 - 1 = 0 \}
        </me>
        which is a hyperbola:
      </p>

      <figure>
        <caption></caption>
        <image>
          <latex-image>
            <![CDATA[\begin{tikzpicture}[domain=-1.2:1.2]
            \draw[<->] (-2,0) -- (2,0) node[below] {\(x\)};
            \draw[<->] (0, -2) -- (0,2) node[right] {\(y\)};
            \draw[very thick] plot[id=p]  ({sinh(\x)}, {cosh(\x)});
            \draw[very thick] plot[id=p]  ({sinh(\x)}, {-cosh(\x)});\end{tikzpicture}]]>
          </latex-image>
        </image>
      </figure>

      <p>
        To show that <m>M</m> is a hypersurface,
        we first compute the gradient of <m>f</m> at a general point <m>\ve{r} = (x,y) \in \mathbb{R}^2</m>:
        <me>
          \nabla_\ve{r} f = (2y, -2x)
        </me>
      </p>

      <p>
        The gradient clearly exists everywhere.
        Moreover, for a point <m>\ve{p} = (a,b)</m> on <m>M</m>, we have
        <me>
          \nabla_\ve{p} f = (2b, -2a)  \text{ where }  b^2 = 1 + a^2
        </me>
      </p>

      <p>
        Suppose <m>\nabla_\ve{p} f = (0,0)</m>.
        Then in particular, <m>2b = 0</m> so that <m>b=0</m>,
        which means that <m>0 = 1 + a^2</m> using the equation for <m>M</m>.
        This is impossible.
        Hence <m>\nabla_\ve{p} f \neq (0,0)</m> for all <m>\ve{p} \in M</m>,
        so that <m>M</m> is a hypersurface.
      </p>
    </solution>
  </example>

  <example>
    <title>Two-sphere</title>
    <statement>
      <p>
        Let <m>f : \mathbb{R}^3 \rightarrow \mathbb{R}</m> be the function
        <me>
          f(x,y,z) = x^2 + y^2 + z^2 -1
        </me>.
      </p>

      <p>
        Draw a picture of the level set <m>M</m> of <m>f</m>,
        and show that it is a differentiable hypersurface.
      </p>
    </statement>
    <solution>
      <p>
        The level set of <m>f</m> is
        <me>
          M = \{ (x,y,z) \in \mathbb{R}^3 : x^2 + y^2 + z^2 - 1 = 0 \}
        </me>
      </p>

      <p>
        This is called the <em>2-sphere</em>,
        and is pictured below:
      </p>

      <figure>
        <caption></caption>
        <image>
          <latex-image>
            <![CDATA[\begin{tikzpicture}\shade[ball color = gray!40, opacity = 0.4] (0,0) circle (2cm);
            \draw (0,0) circle (2cm);
            \draw (-2,0) arc (180:360:2 and 0.6);
            \draw[dashed] (2,0) arc (0:180:2 and 0.6);
            \fill[fill=black] (0,0) circle (1pt);
            \draw[dashed] (0,0) -- (2, 0);
            \draw[->] (2,0) -- node[pos=1.4] {\(y\)} (2.5, 0);
            \draw[dashed] (0,0) --  (0, 2);
            \draw[->] (0,2) -- node[pos=1.4] {\(z\)} (0, 2.5);
            \draw[dashed] (0,0) -- (-0.43, -0.43*4/3);
            \draw[->] (-0.43, -0.43*4/3) -- node[pos=1.2] {\(x\)} (-1.5, -2);\end{tikzpicture}]]>
          </latex-image>
        </image>
      </figure>

      <p>
        To show it is a hypersurface,
        we first compute <m>\nabla f</m> at a general point
        <m>\ve{r} = (x,y,z) \in \mathbb{R}^3</m>:
        <me>
          \nabla_\ve{r} f = (2x, 2y, 2z)
        </me>
      </p>

      <p>
        This clearly exists everywhere.
        Moreover, for a point <m>\ve{p} = (a, b, c)</m>
        on <m>M</m>, we have
        <me>
          \nabla_\ve{p} f = (2a, 2b, 2c) \neq (0, 0, 0)
        </me>
        since <m>a^2 + b^2 + c^2 = 1</m>.
        Hence <m>M</m> is a hypersurface.
      </p>
    </solution>
  </example>

  <example>
    <statement>
      <p>
        Let <m>f : \mathbb{R}^3 \rightarrow \mathbb{R}</m> be the function
        <me>
          f(x,y,z) = (2-\sqrt{x^2 + y^2})^2 + z^2 - 1
        </me>.
      </p>

      <p>
        Draw a picture of the level set <m>M</m> of <m>f</m>,
        and show that it is a hypersurface.
      </p>
    </statement>
    <solution>
      <p>
        The zero set of <m>f</m> is
        <me>
          M = \{ (x,y,z) \in \mathbb{R}^3 : (2-\sqrt{x^2 + y^2})^2 + z^2 - 1 = 0 \}
        </me>
      </p>

      <p>
        This is a <em>torus</em>, and is pictured below:
      </p>

      <figure>
        <caption></caption>
        <image>
          <latex-image>
            <![CDATA[\begin{tikzpicture}\node at (0,0) {\includegraphics[width=0.45\textwidth]{torus.pdf}};
            \draw[->, very thick] (2.5,0) -- node[pos=1.4] {\(y\)} (3.2, 0);
            \draw[->, very thick] (0,0) -- node[pos=1.1] {\(z\)} (0, 2.5);
            \draw[->, very thick] (-0.9, -0.9*4/3) -- node[pos=1.2] {\(x\)} (-1.5, -2);\end{tikzpicture}]]>
          </latex-image>
        </image>
      </figure>

      <p>
        To show <m>M</m> is a hypersurface,
        we first compute <m>\nabla f</m> at a general point
        <m>\ve{r} = (x,y,z) \in \mathbb{R}^3</m>:
        <me>
          \nabla_\ve{r} f = \left( \frac{2x(2 - \sqrt{x^2 + y^2)}}{\sqrt{x^2 + y^2}}, \, \frac{2y(2 - \sqrt{x^2 + y^2)}}{\sqrt{x^2 + y^2}}, \, 2z \right)
        </me>
      </p>

      <p>
        Note that <m>\nabla f</m> doesn't exist
        <em>everywhere</em> in <m>\mathbb{R}^3</m>,
        since there is a problem when
        <m>x^2 + y^2 = 0</m> (i.e. on the <m>z</m>-axis).
        But for a point <m>\ve{p} = (a, b, c)</m> on <m>M</m>,
        we cannot have <m>a^2 + b^2 = 0</m> since that implies,
        using the equation for <m>M</m>, that
        <me>
          (2 - \sqrt{0})^2 + c^2 - 1 = 0
        </me>,
        in other words, <m>c^2 = -3</m> which is impossible.
        So <m>\nabla_\ve{p} f</m> exists everywhere on <m>M</m>.
        Moreover, suppose <m>\nabla_\ve{p} f = (0,0,0)</m> and <m>\ve{p}</m> lies on <m>M</m>.
        Then in particular <m>2c = 0</m> so <m>c=0</m>, and hence,
        using the equation for <m>M</m>,
        <me>
          (2 - \sqrt{a^2 + b^2})^2 = 1
        </me>
        which implies that <m>a</m> and <m>b</m> cannot both be zero.
        This is a contradiction,
        hence <m>\nabla_\ve{p} \neq \ve{0}</m> everywhere on <m>M</m>.
        So <m>M</m> is a hypersurface.
      </p>
    </solution>
  </example>

  <definition>
    <statement>
      <p>
        Let <m>M \subset \mathbb{R}^{n+1}</m> be a hypersurface
        associated to a function <m>f : \mathbb{R}^{n+1} \rightarrow \mathbb{R}</m>.
        The <term>tangent space</term> of <m>M</m> at <m>\ve{p} \in M</m> is:
        <me>
          T_\ve{p} M := \{ \ve{v} \in \mathbb{R}^{n+1} \, : \, \nabla_\ve{p} f \dotp \ve{v} = 0 \}
        </me>
      </p>
    </statement>
  </definition>

  <assemblage>
    <p>
      From Multivariable Calculus,
      you know that we can equivalently express the tangent space to <m>M</m> at <m>p</m> as
      <md>
        <mrow>T_\ve{p} M \amp =  \{ \ve{v} \in \mathbb{R}^{n+1} \, : \, D_\ve{v} f (\ve{p}) = 0 \}</mrow>
        <mrow>\amp =  \left\{ \ve{v} \in \mathbb{R}^{n+1} \, : \, \frac{d}{dt}\Big|_{t=0} f(\ve{p} + t \ve{v}) = 0 \right\}</mrow>
      </md>
    </p>
  </assemblage>

  <lemma>
    <statement>
      <p>
        If <m>M</m>
      </p>
    </statement>
  </lemma>

  <example>
    <statement>
      <p>
        Compute a basis for the tangent space to the hyperbola <m>M</m>
        from <xref ref="hyperbola_example">Example</xref>
        at <m>\ve{p} = (1, \sqrt{2})</m>.
        Draw a picture to illustrate the result.
      </p>
    </statement>
    <solution>
      <p>
        We have already computed the gradient of <m>f</m> at a point <m>\ve{p} = (a,b) \in M</m>:
        <me>
          \nabla_\ve{p} = (2b, -2a)  \text{ where }b^2 = 1 + a^2
        </me>.
      </p>

      <p>
        Hence at <m>\ve{p} = (1, \sqrt{2})</m>, we have
        <me>
          \nabla_\ve{p} f = (2 \sqrt{2}, -2)
        </me>.
      </p>

      <p>
        Thus
        <md>
          <mrow>T_\ve{p} M \amp = \{ (v_1, v_2) \in \mathbb{R}^2 : \nabla_\ve{p} f \dotp (v_1, v_2) = 0 \}</mrow>
          <mrow>\amp = \{ (v_1, v_2) \in \mathbb{R}^2 : 2 \sqrt{2} v_1 - 2v_2 = 0  \}</mrow>
        </md>
      </p>

      <p>
        A basis for <m>T_\ve{p} M</m> is <m>\ve{u} = (1, \frac{1}{\sqrt{2}})</m>.
        The picture is: tikzalign
      </p>

      <figure>
        <caption></caption>
        <image>
          <latex-image>
            <![CDATA[\begin{tikzpicture}[domain=-1.4:1.4]
            \draw[<->] (-2,0) -- (2,0) node[below] {\(x\)};
            \draw[<->] (0, -2) -- (0,2) node[right] {\(y\)};
            \draw[very thick] plot[id=p]  ({sinh(\x)}, {cosh(\x)});
            \draw[very thick] plot[id=p]  ({sinh(\x)}, {-cosh(\x)});
            \draw[very thick, red] plot[id=p] ({1.5*\x}, {1/sqrt(2)*(1.5*\x) + (sqrt(2)-1/sqrt(2))});
            \draw[very thick, fill] (1, 1.414) circle (1pt) node[below right] {\(\ve{p}\)};
            \node at (-1.5, 1.4) {\(M\)};
            \draw[line width=0.5mm, blue, ->] (1, 1.414) -- (1.5, 1.414 + 0.5*0.707) node[below right] {\(\ve{u}\)};\end{tikzpicture}]]>
          </latex-image>
        </image>
      </figure>

      <figure>
        <caption></caption>
        <image>
          <latex-image>
            <![CDATA[\begin{tikzpicture}[domain=-1.4:1.4]
            \draw[<->] (-2,0) -- (2,0) node[below] {\(v_1\)};
            \draw[<->] (0, -2) -- (0,2) node[right] {\(v_2\)};
            \draw[very thick, red] plot[id=p] ({1.5*\x}, {1/sqrt(2)*(1.5*\x)});
            \node[red] at (2, 1.8) {\(T_\ve{p} M\)};
            \draw[line width=0.5mm, blue, ->] (0,0) -- (0.5, 0.5*0.707) node[right, yshift=-2pt] {\(\ve{u}\)};\end{tikzpicture}]]>
          </latex-image>
        </image>
      </figure>

      <p>
        The red line in the first picture,
        drawn for the sake of illustration,
        is the tangent space shifted so that it passes through <m>\ve{p}</m>.
        The actual tangent space <m>T_\ve{p} M</m> goes through the origin as in the second picture.
      </p>

    </solution>
  </example>

</appendix>

