
<section xmlns:xi="http://www.w3.org/2001/XInclude" xml:id="Ch1Sec5ResultsVectorSpace">
  <title>Some results about abstract vector spaces</title>
  <p>
    It is time to use the rules of a vector space to prove some general results.
  </p>

  <assemblage>
    <p>
      We are about to do our first formal proof in the course!
    </p>
  </assemblage>

  <p>Our first lemma shows that the zero vector <m>\ve{0}</m> is the <em>unique</em> vector in <m>V</m> which 'behaves like a zero vector'. More precisely:</p>
  <lemma>
    <statement>
      <p>
        Suppose <m>V</m> is a vector space with zero vector <m>\ve{0}</m>.
        If <m>\ve{0}'</m> is a vector in <m>V</m> satisfying
        <men xml:id="uniqueness_zero">
          \ve{0}' + \ve{v} = \ve{v} \text{ for all }\ve{v} \in V
        </men>
        then <m>\ve{0}' = \ve{0}</m>.
      </p>
    </statement>
  </lemma>

  <proof>
    <md>
      <mrow>\ve{0} \amp = \ve{0}' + \ve{0} \amp \amp \text{using } <xref ref="uniqueness_zero"/> \text{ with } \ve{v}=\ve{0} </mrow>
      <mrow>\amp = \ve{0}' \amp \amp \text{( } <xref ref="R3b">R3b </xref>\text{)}   </mrow>
    </md>
  </proof>

  <definition>
    <statement>
      <p>
        If <m>V</m> is a vector space,
        we define the <term>additive inverse</term>
        of a vector <m>\ve{v} \in V</m> as
        <me>
          - \ve{v} := (-1) \smul\ve{v}
        </me>
      </p>
    </statement>
  </definition>

  <lemma xml:id="add_inv">
    <statement>
      <p>
        If <m>V</m> is a vector space,
        then for all <m>\ve{v} \in V</m>,
        <men>
          -\ve{v} + \ve{v} = \ve{0} \mbox{ and }  \ve{v} + (-\ve{v}) = \ve{0}
        </men>.
      </p>
    </statement>
  </lemma>

  <proof>
    <md>
      <mrow>-\ve{v} + \ve{v} \amp = (-1) \smul\ve{v} + \ve{v} \amp \amp  \mbox{(using defn of \(- \ve{v}\))}</mrow>
      <mrow>\amp = (-1) \smul\ve{v} + 1 \smul\ve{v} \amp \amp  \mbox{(R7)}</mrow>
      <mrow>\amp  = (-1 + 1) \smul\ve{v} \amp \amp  \mbox{(R5)}</mrow>
      <mrow>\amp = 0 \smul\ve{v}</mrow>
      <mrow>\amp = \ve{0} \amp \amp  \mbox{(R8)}</mrow>
    </md>
    <p>
      In addition,
      <md>
        <mrow>\ve{v} + (-\ve{v}) \amp = -\ve{v} + \ve{v} \amp \amp  \mbox{(R1)}</mrow>
        <mrow>\amp  = \ve{0} \amp \amp  \mbox{(by previous proof)}</mrow>
      </md>
    </p>
  </proof>

  <lemma>
    <statement>
      <p>
        Suppose that two vectors <m>\ve{w}</m> and <m>\ve{v}</m> in a vector space satisfy <m>\ve{w} + \ve{v} = \ve{0}</m>.
        Then <m>\ve{w} = -\ve{v}</m>.
      </p>
    </statement>
  </lemma>

  <proof>
    <md>
      <mrow>\ve{w} \amp = \ve{w} + \ve{0} \amp \amp  \mbox{(R3b)}</mrow>
      <mrow>\amp = \ve{w} + (\ve{v} + -\ve{v}) \amp \amp  \mbox{by } <xref ref="add_inv"/></mrow>
      <mrow>\amp = (\ve{w} + \ve{v}) + -\ve{v}) \amp \amp  \mbox{(R2)}</mrow>
      <mrow>\amp = \ve{0} + -\ve{v} \amp \amp  \mbox{(by assumption)}</mrow>
      <mrow>\amp = -\ve{v} \amp \amp  \mbox{(R3a)} </mrow>
    </md>.
  </proof>

  <p>
    Let us prove two more lemmas, for practice. 
  </p>

  <lemma xml:id="scalar_times_zero_vec">
    <statement> 
      <p>
      Let <m>V</m> be a vector space and <m>k</m> any scalar. Then
      <me>
        k \smul\ve{0} = \ve{0}
      </me>
     </p>
    </statement>
  </lemma>
  <proof>
    <md>
      <mrow> k \smul\ve{0} \amp = k \smul(0 \smul\ve{0}) \amp \text{(R8 for } \ve{v}=\ve{0}\text{)} </mrow>
      <mrow> \amp = ((k)(0))\smul\ve{0} \amp \text{(R6)} </mrow>
      <mrow> \amp = 0 \smul\ve{0} \amp \text{(} (k)(0)=0 \text{ for any real number }  k \text{)} </mrow>
      <mrow> \amp = \ve{0} \amp \text{(R8 for } \ve{v}=\ve{0}\text{)} </mrow>
    </md>
  </proof>

  <lemma xml:id="dichotomy_lem">
    <statement>
      <p>
        Suppose that <m>\ve{v}</m> is a vector in a vector space <m>V</m> and that <m>k</m> is a scalar.
        Then
        <me>
          k \smul\ve{v} = \ve{0}  \Leftrightarrow  k = 0 \mbox{ or }  \ve{v} = \ve{0}
        </me>.
      </p>
    </statement>
  </lemma>

  <proof>
    <p>
      <alert>(Proof of <m>\Leftarrow</m>)</alert>.
      Suppose <m>k=0</m>.
      Then <m>k \smul\ve{v} = 0 \smul\ve{v} = \ve{0}</m> by R8 of a vector space.
      On the other hand, suppose <m>\ve{v} = \ve{0}</m>.
      Then <m>k \smul\ve{v} = k \smul\ve{0} = \ve{0}</m> by <xref ref="mult_by_zero_ex">Exercise</xref>.
    </p>

    <p>
      (Proof of <m>\Rightarrow</m>).
      Suppose <m>k \smul\ve{v} = \ve{0}</m>.
      There are two possibilities:
      either <m>k = 0</m>, or <m>k \neq 0</m>.
      If <m>k=0</m>, then we are done.
      If <m>k \neq 0</m>,
      then <m>\frac{1}{k}</m> exists and we can multiply both sides by it:
      <md>
        <mrow>k \smul\ve{v} \amp  = \ve{0}</mrow>
        <mrow>\therefore  \frac{1}{k} \smul(k \smul\ve{v})  \amp  = \frac{1}{k} \smul\ve{0} \amp \amp  \mbox{(Multiplied both sides by \(\frac{1}{k}\))}</mrow>
        <mrow>\therefore \left(\frac{1}{k} k\right) \smul\ve{v} \amp = \ve{0} \amp \amp  \mbox{(On the LHS, we used R6. On the RHS, we used } <xref ref="mult_by_zero_ex"/>)</mrow>
        <mrow>\therefore 1 \smul\ve{v} \amp = \ve{0} \amp \amp  \mbox{(using \(\frac{1}{k} k = 1\))}</mrow>
        <mrow>\therefore \ve{v} \amp = \ve{0} \amp \amp  \mbox{(R7)}</mrow>
      </md>
    </p>

    <p>
      Hence in the case <m>k \neq 0</m> we must have <m>\ve{v} = \ve{0}</m>,
      which is what we wanted to show.
    </p>
  </proof>

  <example xml:id="explicit_solve_x">
      <p>
        Let us practice using the rules of a vector space to perform everyday calculations.
        For instance,
        suppose that we are trying to solve for the vector <m>\ve{x}</m> appearing in the following equation:
        <men>
          \ve{v} + 7 \smul\ve{x} = \ve{w}
        </men>
      </p>

      <p>
        We do this using the rules as follows:
        <md>
          <mrow>\ve{v} + 7 \smul\ve{x} \amp  = \ve{w}</mrow>
          <mrow>\therefore  -\ve{v} + (\ve{v} + 7 \smul\ve{x}) \amp  = -\ve{v} + \ve{w} \amp \amp  \mbox{(Added \(-\ve{v}\) on left to both sides)}</mrow>
          <mrow>\therefore  (-\ve{v} + \ve{v}) + 7 \smul\ve{x} \amp  = -\ve{v} + \ve{w} \amp \amp  \mbox{(used R2 on LHS)}</mrow>
          <mrow>\therefore  \ve{0} + 7 \smul\ve{x} \amp  = -\ve{v} + \ve{w} \amp \amp  \mbox{(used } <xref ref="add_inv"/> \mbox{ on LHS)}</mrow>
          <mrow>\therefore  7 \smul\ve{x} \amp  =  -\ve{v} + \ve{w} \amp \amp  \mbox{(used R3a on LHS)}</mrow>
          <mrow>\therefore  \frac{1}{7} \smul(7 \smul\ve{x}) \amp  = \frac{1}{7} \smul(-\ve{v} + \ve{w}) \amp \amp  \mbox{(scalar multiplied both sides by \(\frac{1}{7}\))}</mrow>
          <mrow>\therefore  (\frac{1}{7} 7) \smul  \ve{x} \amp  = \frac{1}{7} \smul(-\ve{v} + \ve{w}) \amp \amp  \mbox{(used R6 on LHS)}</mrow>
          <mrow>\therefore  1 \smul\ve{x} \amp  =  \frac{1}{7} \smul(-\ve{v} + \ve{w})  \amp \amp  \mbox{(multiplied \(\frac{1}{7}\) with \(7\))}</mrow>
          <mrow>\therefore  \ve{x} \amp  =  \frac{1}{7} \smul(-\ve{v} + \ve{w}) \amp \amp  \mbox{(R7)}</mrow>
        </md>
      </p>

      <p>
        As the course goes on we will leave out all these steps.
        But it is important for you to be able to reproduce them all,
        if asked to do so!
      </p>

  </example>



<exercises>
  <exercise xml:id="minus_minus_v_equals_v">
    <statement>
      <p>
        Prove that for all vectors <m>\ve{v}</m> in a vector space,
        <m>-(-\ve{v}) = \ve{v}</m>.
      </p>
    </statement>
    <solution>
      <p>
        We apply the definition of <m>-\ve v</m> twice:
        <me>
        -(-\ve{v}) = (-1)\smul(- \ve v) = (-1)\smul(-1\smul(\ve v)).
      </me>
      Using <xref ref="R6"/> we get
      <me>
(-1)\smul(-1(\ve v)) = ((-1)(-1))\smul\ve v = 1.\ve v.
    </me>
    Finally, a single application of <xref ref="R7"/> allows us to conclude that
    <me>
1.\ve v = \ve v
  </me>
      </p>
    </solution>
  </exercise>

  <exercise xml:id="mult_by_zero_ex">
    <statement>
      <p>
        Let <m>V</m> be a vector space with zero vector <m>\ve{0}</m>.
        Prove that for all scalars <m>k</m>,
        <m>k \smul \ve{0} = \ve{0}</m>.
      </p>
    </statement>
      <solution>
        <p>
          We apply <xref ref = "R3b"/> to <m>k \smul \ve{0}</m>:
          <me>
k \smul \ve{0} = k \smul (\ve 0 + \ve 0).
        </me>
        By <xref ref = "R4"/> we get
        <me>
        k \smul (\ve 0 + \ve 0) = k \smul \ve 0 + k \smul 0.
      </me>
      We now know
      <me>
k \smul \ve{0} = k \smul \ve 0 + k \smul 0.
    </me>
    Adding the inverse of <m>k \smul 0</m> to both sides we get
    <me>
\ve 0 = k \smul \ve 0 + \ve 0 = k \smul 0.
  </me>
  And we are done.
        </p>
        </solution>
  </exercise>

  <exercise xml:id="fivevequals2v">
    <statement>
    <p>
      Let <m>V</m> be a vector space. Suppose that a vector <m>\ve{v} \in V</m> satisfies
      <men xml:id="funny-eqn-smul">
        5\smul \ve{v} = 2 \smul \ve{v}.
      </men>
      Prove that <m>\ve{v}=\ve{0}</m>.
    </p>
  </statement>
        <solution>
        <p>
          <md>
            <mrow>\amp  5 \smul v = 2\smul v </mrow>
          <mrow> \amp \implies 5.v + (-2).v = 2.v + (-2).v </mrow>
          <mrow>\amp \implies (5 - 2).v = (2 - 2).v </mrow>
          <mrow> \amp \implies 3.v = 0.v </mrow>
          <mrow> \amp \implies (\frac{1}{3} 3).v = (\frac{1}{3} 0) v </mrow>
          <mrow> \amp \implies 1v = 0v </mrow>
          <mrow> \amp \implies v = 0</mrow>
        </md>
        </p>
      </solution>
  </exercise>

  <exercise xml:id="solve_for_x_exercise">
    <statement>
      <p>
        Suppose that two vectors <m>\ve{x}</m> and <m>\ve{w}</m> in a vector space satisfy <m>2 \ve{x} + 6 \ve{w} = \ve{0}</m>.
        Solve for <m>\ve{x}</m>,
        showing explicitly how you use the rules of a vector space,
        as in <xref ref="explicit_solve_x"/>.
      </p>
    </statement>
    <solution>
      <p>
        <md>
         <mrow>2 \ve x + 6 \ve w  \amp = \ve 0</mrow>

          <mrow>\implies  2 \ve x + 6 \ve w + (-6 \ve w )\amp  \ve 0 + (-6\ve w) 
           \amp (\text{Existence of Inverses})</mrow>

          <mrow> \implies  2 \ve x + 0  \amp = -6\ve w  \amp (<xref ref = "R3a"> R3a </xref>)</mrow>

           <mrow> \implies  2\ve x   \amp = -6\ve w  \amp (<xref ref = "R3b"> R3b </xref>)</mrow>

           <mrow> \implies  (\frac{1}{2})(2 \ve x) \amp = ((\frac{1}{2}))(-6\ve w)  </mrow>

            <mrow> \implies  (\frac{1}{2}2)\ve x  \amp = (-\frac{1}{2}6)\ve w) \amp (<xref ref = "R6"> R6 </xref>)</mrow>

               <mrow>\implies   1 \ve x  \amp  = -3 \ve w  </mrow>

                <mrow>\implies  \ve x   \amp = -3 \ve w  \amp (<xref ref = "R7"> R7 </xref>) </mrow>
                </md>
</p>
</solution>
  </exercise>

  <exercise>
    <statement>
    <p>
      Suppose <m>V</m> is a vector space which is not the zero vector space. Show that <m>V</m> contains infinitely many elements.
    </p>
  </statement>
  <hint xml:id="inf-elements-hint1">
    <p>
      Since <m>V</m> is not the zero vector space, there must exist a vector <m>\ve{v} \in V</m> such that <m>\ve{v} \neq \ve{0}</m>.
    </p>
  </hint>
  <hint>
    <p>
      Use the idea of the proof from <xref ref="fivevequals2v"/>.
    </p>
  </hint>
  </exercise>

  <exercisegroup>
    <title>True or False</title>
    <introduction>
      <p>
      For each of the following statements, write down whether the statement is true or false, and prove your assertion. (In other words, if you say that it is true, prove that it is true, and if you say that it is false, prove that it is false, by giving an <em>explicit counterexample</em>.)
      </p>
    </introduction>
    <exercise xml:id="is_k_equal_to_zero">
      <statement>
      <p>
        If <m>k \smul \ve{v} = \ve{0}</m> in a vector space, then it necessarily follows that <m>k=0</m>.
      </p>
    </statement>
    <solution>
      <p>
        False. Take <m>\mathbb{R}^2</m> as an example. If <m>v = (0,0)</m> then
        <m>2.(0,0) = (0,0) </m> but, of course, <m> 2 \neq 0</m>.
      </p>
      </solution>
    </exercise>
    <exercise>
      <statement>
      <p>
        If <m>k \smul \ve{v} = \ve{0}</m> in a vector space, then it necessarily follows that <m>\ve{v}=\ve{0}</m>.
      </p>
    </statement>
    </exercise>

    <exercise xml:id="empty_vector_space">
      <statement>
      <p>
        The empty set can be equipped with data <xref ref="D1">D1</xref>, <xref ref="D2">D2</xref>, <xref ref="D3">D3</xref> satisfying the rules of a vector space.
      </p>
    </statement>
     <solution>
    <p>
      False. In order for the empty set to be a vector space, it must have a zero vector. That is, we must be able to find some <m> v \in \text{the empty set} </m> satisfying the axioms for the zero vector. However, since the empty set has no elements in it, by definition, we cannot ever hope to find such a <m> v </m>. Hence the empty set can never be a vector space.
    </p>
    </solution>
    </exercise>
    
    <exercise>
      <statement>
      <p>
      Rule <xref ref="R3b">R3b</xref> of a vector space follows automatically from the other rules.
      </p>
    </statement>
     <solution>
      True. Combining <xref ref = "R1">R1</xref> and <xref ref = "R3a">R3a</xref> gives <xref ref="R3b">R3b</xref>.
    </solution>
    </exercise>

    <exercise xml:id="R7_follows">
      <statement>
      <p>
      Rule <xref ref="R7">R7</xref> of a vector space follows automatically from the other rules.
      </p>
    </statement>
      <solution>
      <p>
        False. Let <m>V</m> be a non-zero vector space (such as <m>\mathbb{R}^2</m>). Redefine scalar multiplication as follows
        <me> 
            k.v := 0 \mbox{ for all scalars k and all vectors v}.
        </me>
        Then <m>V</m> will satisfy all the rules of a vector space except R7. Thus it is not the case that R7 follows from the other rules.
      </p>
      </solution>
    </exercise>

  </exercisegroup>


</exercises>

<solutions divisional="solution answer" />





</section>

