

<section xml:id="Ch3Sec3Isomorphisms">
  <title>Isomorphisms of vector spaces</title>
  <p>
    Suppose you have two sets,
    <me>
      A = \{ \mbox{bird} , \mbox{eye} , \mbox{person}  \}  \mbox{and}    B = \left\{ \begin{aligned}<image width="100%" source="images/bird.png" /> 
      \end{aligned}  , \begin{aligned}<image width="100%" source="images/eye.png" /> 
      \end{aligned} , \begin{aligned}<image width="100%" source="images/person.png" /> 
      \end{aligned}  \right\}
    </me>.
  </p>

  <p>
    The elements of <m>A</m> and <m>B</m> are not <em>the same</em>,
    so <m>A</m> is not <em>equal</em> to <m>B</m>.
    But this is unsatisfactory <mdash /> clearly the elements of <m>A</m> are just English versions of the Chinese symbols in <m>B</m>.
    How can we make this mathematically precise?
  </p>

  <p>
    We could define two maps, say
    <md>
      <mrow>S: A \amp \rightarrow B</mrow>
      <mrow>\mbox{bird}  \amp \mapsto \begin{aligned}<image width="100%" source="images/bird.png" /> 
      \end{aligned}</mrow>
      <mrow>\mbox{eye}  \amp \mapsto \begin{aligned}<image width="100%" source="images/eye.png" /> 
      \end{aligned}</mrow>
      <mrow>\mbox{cross}  \amp \mapsto \begin{aligned}<image width="100%" source="images/person.png" /> 
      \end{aligned}</mrow>
      <intertext>and</intertext>
      <mrow>T : B \amp \rightarrow A</mrow>
      <mrow>\begin{aligned}<image width="100%" source="images/bird.png" /> 
      \end{aligned}  \amp  \mapsto \mbox{bird}</mrow>
      <mrow>\begin{aligned}<image width="100%" source="images/eye.png" /> 
      \end{aligned}  \amp  \mapsto \mbox{eye}</mrow>
      <mrow>\begin{aligned}<image width="100%" source="images/person.png" /> 
      \end{aligned}  \amp  \mapsto \mbox{cross}  </mrow>
    </md>.
  </p>

  <p>
    Then we observe that
    <men xml:id="bijection_eqn">
      T \circ S = \id_A  \mbox{and}   S \circ T = \id_B 
    </men>.
  </p>

  <p>
    A pair of maps <m>S : A \rightarrow B</m> and
    <m>T : B \rightarrow A</m> satisfying <xref ref="bijection_eqn" /> is called an
    <em>isomorphism of sets</em>
    between <m>A</m> and <m>B</m>.
    If you like,
    you can rename <m>T</m> as <m>S^{-1}</m> since <m>S^{-1} \circ S = \id_A</m> and
    <m>S \circ S^{-1} = \id_B</m>. (Calling <m>T</m> by the name <m>S^{-1}</m> from the beginning would have been presumptive of me.
    I needed to first define it,
    and then check that it satisfied <xref ref="bijection_eqn" />.
    Only then did I have the right to call it <m>S^{-1}</m>!)
  </p>

  <p>
    Perhaps you are somewhat of a penny-pincher.
    You see the need for the English-to-Chinese map <m>S</m>,
    but not the need for a Chinese-to-English map <m>T</m>.
    After all, you say,
    since no two different English symbols in <m>A</m> get mapped to the same Chinese symbol in <m>B</m> (<sq><m>S</m> is one-to-one</sq>) and every Chinese symbol <m>y \in B</m> is equal to <m>S(x)</m> for some <m>x \in A</m> (<sq><m>S</m> is onto</sq>),
    we have no need for <m>T</m>.
    It is an extravagance!
  </p>

  <p>
    To this I respond: you are right,
    but is it not useful to have the explicit Chinese-to-English map <m>T</m>?
    In bookshops,
    cross-language dictionaries like this most often come bundled as a pair,
    in a single volume.
    After all, if one needs to look up the English word for <m>\begin{aligned}<image width="100%" source="images/bird.png" /> 
    \end{aligned}</m>,
    it is a nuisance to have to traverse through the entire English-to-Chinese dictionary,
    trying to find the English word which translates to <m>\begin{aligned}<image width="100%" source="images/bird.png" /> 
    \end{aligned}</m>!
  </p>

  <p>
    This motivates the following definition.
  </p>

  <definition>
    <statement>
      <p>
        We say that a linear map <m>S : V \rightarrow W</m> is an <term>isomorphism</term>
        if there exists a linear map <m>T : W \rightarrow V</m> such that
        <men xml:id="inverse_map_in_iso">
          T \circ S = \id_V  \mbox{and}   S \circ T = \id_W
        </men>.
      </p>
    </statement>
  </definition>

  <lemma>
    <title>Uniqueness of Inverses</title>
    <statement>
      <p>
        If <m>S : V \rightarrow W</m> is an isomorphism and <m>T, T' : W \rightarrow V</m> both satisfy
        <md>
          <mrow>T \circ S \amp = \id_V, \ \amp  S \circ T \amp = \id_W</mrow>
          <mrow>T' \circ S \amp = \id_V, \ \amp  S \circ T' \amp = \id_W</mrow>
        </md>
        then <m>T = T'</m>.
      </p>
    </statement>
  </lemma>

  <assemblage>
    <p>
      This lemma justifies us calling <m>T</m>
      <em>the</em> inverse of <m>S</m>
      (as opposed to <em>an</em> inverse of <m>S</m>),
      and also justifies us writing <m>T = S^{-1}</m>.
    </p>
  </assemblage>

  <proof>
    <p>
      To show that <m>T = T'</m>,
      we must show that for all <m>\ve{w} \in W</m>,
      <m>T(\ve{w}) = T'(\ve{w})</m>.
      Indeed:
      <md>
        <mrow>T(\ve{w}) \amp = T(\id_W (\ve{w})) \amp \amp  \mbox{(Defn of \(\id_W\))}</mrow>
        <mrow>\amp = T( (S \circ T')(\ve{w})) \amp \amp  \mbox {($S \circ T' = \id_W$)}</mrow>
        <mrow>\amp = T(S(T'(\ve{w}))) \amp \amp  \mbox {(Defn of $S \circ T'$)}</mrow>
        <mrow>\amp = (T \circ S)(T'(\ve{w})) \amp \amp  \mbox {(Defn of $T \circ S$)}</mrow>
        <mrow>\amp = \id_V (T'(\ve{w})) \amp \amp  \mbox{(\(T \circ S = \id_V\))}</mrow>
        <mrow>\amp = T'(\ve{w}) \amp \amp  \mbox {(Defn of $\id_V$)}</mrow>
      </md>.
    </p>
  </proof>

  <definition>
    <statement>
      <p>
        We say that two vector spaces <m>V</m> and <m>W</m> are <term>isomorphic</term>
        if there exists an isomorphism between them.
      </p>
    </statement>
  </definition>

  <example>
    <statement>
    <p>
      Show that <m>\mathbb{R}^n</m> is isomorphic to <m>\Poly_{n-1}</m>
    </p>
    <p>
    <solution>
      <p>
        We define a pair of linear maps
        <md>
          <mrow>S : \mathbb{R}^n \amp  \rightleftarrows \Poly_{n-1} : T</mrow>
          <intertext>as follows:</intertext>
          <mrow>(a_1, a_2, \ldots, a_n) \amp  \stackrel{S}{\mapsto} a_1 + a_2 x + \cdots + a_n x^{n-1}</mrow>
          <mrow>(a_1, a_2, \ldots, a_n) \amp  \stackrel{T}{\mapsfrom} a_1 + a_2 x + \cdots + a_n x^{n-1}</mrow>
        </md>
      </p>
    </solution>
</p>
   
    <p>
      We clearly have <m>T \circ S = \id_{\mathbb{R}^n}</m> and <m>S \circ T = \id_{\Poly_{n-1}}</m>.
    </p>
    </statement>
  </example>

 <exercise>
      <statement>
        <p>
          Check that these maps are linear.
        </p>
      </statement>
    </exercise>


  <p>
    We will now show that up to isomorphism,
    there is only one vector space of each dimension!
  </p>

  <theorem xml:id="iso_same_dim">
    <statement>
      <p>
        Two finite-dimensional vector spaces <m>V</m> and <m>W</m> are isomorphic if and only if they have the same dimension.
      </p>
    </statement>
  </theorem>

  <proof>
    <p>
      <m>\Rightarrow</m>.
      Suppose <m>V</m> and <m>W</m> are isomorphic,
      via a pair of linear maps <m>S : V \rightleftarrows W : T</m>.
      Let <m>\basis{B} = \bopen \ve{e}_1, \ldots, \ve{e}_m \bclose</m> be a basis for <m>V</m>.
      Then I claim that <m>\basis{C} = \bopen S(\ve{e}_1), \ldots, S(\ve{e}_m) \bclose</m> is a basis for <m>W</m>.
      Indeed, the list of vectors
      <m>\basis{C}</m> is linearly independent, since if
      <me>
        a_1 S(\ve{e}_1) + a_2 S(\ve{e}_2) + \cdots + a_m S(\ve{e}_m) = \ve{0}_W
      </me>,
      then applying <m>T</m> to both sides we obtain
      <md>
        <mrow>T(a_1 S(\ve{e}_1) + a_2 S(\ve{e}_2) + \cdots + a_m S(\ve{e}_m)) \amp  = T(\ve{0}_W)</mrow>
        <mrow>\therefore a_1 T(S(\ve{e}_1)) + a_2 T(S(\ve{e}_2)) + \cdots + a_m T(S(\ve{e}_m)) \amp = \ve{0}_V \amp \amp  \mbox{(\(T\) is linear)}</mrow>
        <mrow>\therefore a_1 \ve{e}_1 + a_2 \ve{e}_2 + \cdots + a_m \ve{e}_m \amp = \ve{0}_V \amp \amp  \mbox{(\(T\circ S = \id_V\))}</mrow>
      </md>
      which implies that <m>a_1 = a_2 = \cdots = a_m = 0</m>,
      since <m>\basis{B}</m> is linearly independent.
      Moreover, the list of vectors <m>\basis{C}</m> spans <m>W</m>,
      for if <m>\ve{w} \in W</m>, then applying <m>T</m>, we can write
      <me>
        T(\ve{w}) = a_1 \ve{e}_1 + a_2 \ve{e}_2 + \cdots + a_m \ve{e}_m
      </me>
      for some scalars <m>a_i</m> since <m>\basis{B}</m> spans <m>V</m>.
      But then
      <md>
        <mrow>\ve{w} \amp = S(T(\ve{w})) \amp \amp  \mbox{(since \(S \circ T = \id_W\))}</mrow>
        <mrow>\amp = S(a_1 \ve{e}_1 + a_2 \ve{e}_2 + \cdots + a_m \ve{e}_m)</mrow>
        <mrow>\amp = a_1 S(\ve{e}_1) + a_2 S(\ve{e}_2) + \cdots + a_m S(\ve{e}_m) \amp \amp  \mbox{(\(S\) is linear)}</mrow>
      </md>
      so that <m>\basis{C}</m> spans <m>W</m>.
      Hence <m>\basis{C}</m> is a basis for <m>V</m>,
      so <m>\Dim V = \mbox{number of vectors in <m>\basis{B}</m>}</m> = <m>m</m>,
      while <m>\Dim W = \mbox{number of vectors in <m>\basis{C}</m>}  = m</m>.
    </p>

    <p>
      <m>\Leftarrow</m>.
      Suppose <m>\Dim V = \Dim W</m>.
      Let <m>\ve{e}_1, \ldots, \ve{e}_m</m> be a basis for <m>V</m>,
      and let <m>\ve{f}_1, \ldots, \ve{f}_m</m> be a basis for <m>W</m>.
      (We know that the number of basis vectors is the same since <m>\Dim V = \Dim W</m>.)
    </p>

    <p>
      To define linear maps
      <md>
        <mrow>S : V \amp \rightleftarrows W : T</mrow>
        <intertext>it is sufficient, by <xref ref="defining_linear_map_on_basis">Proposition</xref> (Sufficient to Define a Linear Map on a Basis), to define the action of <m>S</m> and <m>T</m> on the basis vectors. We set:</intertext>
        <mrow>\ve{e}_i \amp  \stackrel{S}{\mapsto} \ve{f}_i</mrow>
        <mrow>\ve{e}_i \amp  \stackrel{T}{\mapsfrom} \ve{f}_i</mrow>
      </md>
    </p>

    <p>
      Clearly we have <m>T \circ S = \id_V</m> and <m>S \circ T = \id_W</m>.
    </p>
  </proof>

  <example>
    <statement>
      <p>
        Show that <m>\Mat_{n,m}</m> is isomorphic to <m>\mathbb{R}^{mn}</m>.
      </p>
    </statement>
    <solution>
      <p>
        We simply observe that by <xref ref="dimension_of_matrix_space_example">Example</xref>,
        <m>\Dim \Mat_{n,m} = mn</m> while
        from <xref ref="standard_basis_R_n_ex">Example</xref>,
        <m>\Dim \mathbb{R}^{mn}</m> is also equal to <m>mn</m>.
      </p>
    </solution>
  </example>

  <p>
    There is one very important isomorphism which we will use over and over.
    Let <m>V</m> be a vector space with basis <m>\basis{B} = \bopen \ve{b}_1, \ldots, \ve{b}_m \bclose</m>.
    Consider the map
    <md>
      <mrow>_\basis{B} : V \amp  \rightarrow \Col_m</mrow>
      <mrow>\ve{v} \amp  \mapsto [\ve{v}]_\basis{B}</mrow>
    </md>
    which sends a vector <m>\ve{v} \in V</m> to its corresponding coordinate vector <m>[\ve{v}]_\basis{B} \in \Col_m</m>.
    <xref ref="lin_of_coord_vectors">Lemma</xref>
    says precisely that <m>[ \smul]_\basis{B}</m> is a linear map.
    We will now describe its inverse.
  </p>

  <definition>
    <statement>
      <p>
        Let <m>V</m> be an <m>m</m>-dimensional vector space with basis <m>\basis{B} = \bopen \ve{e}_1, \ldots, \ve{e}_m\bclose</m>.
        Let <m>\mat{c} \in \Col_m</m> be an <m>m</m>-dimensional column vector.
        Then the <term>vector in <m>V</m> corresponding to <m>\mat{c}</m> with respect to the basis <m>\basis{B}</m></term> is
        <me>
          \ve{vec}_{V, \basis{B}} (\mat{c}) := \mat{c}_1 \ve{e}_1 + \mat{c}_2 \ve{e}_2 + \cdots + \mat{c}_m \ve{e}_m
        </me>.
      </p>
    </statement>
  </definition>

  <example>
    <statement>
      <p>
        The polynomials <m>\basis{B} = \bopen \ve{p}_1, \ve{p}_2, \ve{p}_3 \bclose</m> where
        <me>
          \ve{p}_1 := 1 + x,  \ve{p}_2 := 1 + x + x^2, \ve{p}_3 := 1-x^2
        </me>
        are a basis of <m>\Poly_2</m>
        (check this).
        Then, for instance,
        <md>
          <mrow>\ve{vec}_{\Poly_3, \basis{B}} \left( \begin{bmatrix}  2 \\ -3 \\ 3\end{bmatrix}\right) \amp = 2(1+x) -3 (1+x+x^2) + 3(1-x^2)</mrow>
          <mrow>\amp =  2 -x -6x^2 \in \Poly_3 \, </mrow>
        </md>.
      </p>
    </statement>
  </example>

  <exercise>
    <statement>
      <p>
        Show that:

        <ol>
          <li>
            
            <p>
              <m>\ve{vec}_{V, \basis{B}} (\mat{c} + \mat{c}') = \ve{vec}_{V, \basis{B}} (\mat{c}) + \ve{vec}_{V, \basis{B}} (\mat{c}')</m>
            </p>
          </li>

          <li>
           
            <p>
              <m>\ve{vec}_{V, \basis{B}} (k\mat{c}) = k \, \ve{vec}_{V, \basis{B}} (\mat{c})</m>.
            </p>
          </li>
        </ol>
      </p>

      <p>
        This means that <m>\ve{vec}_{V, \basis{B}} : \Col_m \rightarrow V</m> is a linear map.
      </p>
    </statement>
    <solution>
      <p>
 <ol>
          <li>
             <p>
              <md>
              <mrow>\ve{vec}_{V, \basis B}(\mat c + \mat c') \amp = \ve{vec}_{V, \basis B}\left( \begin{bmatrix}  c_1 \\ \vdots \\c_n\end{bmatrix} +  \begin{bmatrix}  c^\prime_1\\ \vdots \\ c^\prime_n\end{bmatrix}\right) </mrow>

              <mrow>\amp = \ve{vec}_{V, \basis B}\left( \begin{bmatrix}  c_1+ c^\prime_1 \\ \vdots \\c_n + c^\prime_n \end{bmatrix}\right) </mrow>

              <mrow>\amp =  (c_1+ c^\prime_1)\ve e_1 +\cdots +  (c_n+ c^\prime_n)\ve e_n  </mrow>

              <mrow> \amp = (c_1\ve e_1 + \cdots + c_n\ve e_n )  + (c_1^\prime\ve e_1 + \cdots + c^\prime_n\ve e_n ) </mrow>

              <mrow> \amp = \ve{vec}_{V, \basis B}(\mat c) + \ve{vec}_{V, \basis B}(\mat c')</mrow>

            </md>

            </p>
          </li>

          <li>
            <p>
             <md>

              <mrow>\ve{vec}_{V, \basis B}(k\mat c) \amp = \ve{vec}_{V, \basis B}\left(k \begin{bmatrix}  c_1 \\ \vdots \\c_n\end{bmatrix} \right)  </mrow> 

              <mrow> \amp =  \ve{vec}_{V, \basis B}\left(\begin{bmatrix}  kc_1 \\ \vdots \\kc_n\end{bmatrix} \right)</mrow>

              <mrow> \amp = (kc_1\ve e_1 + \cdots + kc_n\ve e_n )</mrow>

              <mrow> \amp = k(c_1\ve e_1 + \cdots + c_n\ve e_n ) </mrow>

              <mrow> \amp = k\,\ve{vec}_{V, \basis B}(\mat c) </mrow>

             </md>
            </p>
          </li>
        </ol>


</p>
</solution>
        </exercise>

  <theorem>
    <statement>
      <p>
        Let <m>V</m> be a vector space with basis <m>\basis{B} = \bopen \ve{e}_1, \ldots, \ve{e}_m\bclose</m>.
        The maps
        <md>
          <mrow>_\basis{B} : V \amp  \rightleftarrows  \Col_m : \ve{vec}_{V, \basis{B}}</mrow>
          <mrow>\ve{v} \amp  \mapsto [\ve{v}]_{\basis{B}}</mrow>
          <mrow>\ve{vec}_{V, \basis{B}}(\mat{c}) \amp  \mapsfrom \mat{c}</mrow>
        </md>
        are an isomorphism of vector spaces.
      </p>
    </statement>
  </theorem>

  <proof>
    <p>
      Given <m>\ve{v} \in V</m>, expand it in the basis <m>\basis{B}</m>:
      <me>
        \ve{v} = a_1 \ve{e}_1 + \ldots + a_m \ve{e}_m 
      </me>.
    </p>

    <p>
      Then
      <md>
        <mrow>(\ve{vec}_{V, \basis{B}} \circ [\cdot]_\basis{B} ) \big(\ve{v}\big) \amp = \ve{vec}_{V, \basis{B}} \big( [\ve{v}]_\basis{B} \big)</mrow>
        <mrow>\amp = \ve{vec}_{V,\basis{B}} \left( \begin{bmatrix} a_1 \\ \vdots \\ a_m \end{bmatrix} \right)</mrow>
        <mrow>\amp = a_1 \ve{e}_1 + \cdots + a_m \ve{e}_m</mrow>
        <mrow>\amp = \ve{v}</mrow>
      </md>
      so that <m>\ve{vec}_{V, \basis{B}} \circ [\cdot]_\basis{B} = \id_V</m>.
      Conversely, given
      <me>
        \mat{c} = \begin{bmatrix} c_1 \\ \vdots \\ c_m \end{bmatrix}\in \Col_m
      </me>,
      we have
      <md>
        <mrow>\big( [ \smul]_\basis{B} \circ \ve{vec}_{V, \basis{B}} \big)  \big( \mat{c} \big) \amp = 
        \big[\ve{vec}_{V, \basis{B}} (\mat{c}) \big]_\basis{B}</mrow>
        <mrow>\amp = \big[ \mat{c}_1 \ve{e}_1 + \cdots + \mat{c}_m \ve{e}_m \big]</mrow>
        <mrow>\amp = \begin{bmatrix} c_1 \\ \vdots \\ c_m \end{bmatrix}</mrow>
        <mrow>\amp = \mat{c}</mrow>
      </md>
      where the second last step uses the <em>definition</em>
      of the coordinate vector of <m>\ve{v} = \mat{c}_1 \ve{e}_1 + \cdots + \mat{c}_m \ve{e}_m</m>.
      Hence <m>[\cdot]_\basis{B} \circ \ve{vec}_{V, \basis{B}} = \id_{\Col_m}</m>.
    </p>
  </proof>

  <assemblage>
    <p>
      The result above is very important in linear algebra.
      It says that,
      once we have chosen a basis for an abstract finite-dimensional vector space <m>V</m>,
      we can treat the elements of <m>V</m> as if they were column vectors!
    </p>
  </assemblage>
<exercises>
   <exercise>
    <statement>
      <p>
        Are the following vector spaces isomorphic?
       <md>
         <mrow> V \amp = \left\{ \mat{v} \in \Col_4 : \begin{bmatrix} 1 \mamp  2 \mamp  0 \mamp  -1 \\ -1 \mamp  1 \mamp  1 \mamp  0 \end{bmatrix}  \mat{v}  = \mat{0}  \right\} </mrow>
      
        
          <mrow>W \amp = \left\{ p \in \Poly_2 : \int_0^2 p(x) dx = 0 \right\} </mrow>
             </md>.
      </p>

      <p>
        If they are, construct an explicit isomorphism between them.
        If not, prove that they are not isomorphic.
      </p>
    </statement>
    <solution>
      <p>
        V consists of all vectors <m>(x,y,z,w)</m> satisyfing the linear equations
        <md>

         <mrow> x + 2y - w = 0 </mrow>

         <mrow> -x + y + z = 0 </mrow>

        </md>.

        We are free to choose <m>x</m> and <m> y </m> arbitrarily, but then (1) above fixes <m> w </m> and (2) fixes <m> z </m>. Hence <m> V </m> is a 2 dimensional subspace.
      </p>
<p>
Onto <m>W</m>. Let <m>p(x) = ax^2 + bx +c</m>. For <m> p(x) </m> to be in <m> W</m>, <m> p(x)</m> must satisfy the following equation:

      
        <me> 
\int_0^2 ax^2 + bx + c \, dx = \frac{8a}{3} + 2b + 2c = 0.
      </me>
     Thus, for any choice of <m> a </m> and <m> b </m>, <m> c </m> is uniquely determined. Hence <m>W</m> is a 2 dimensional subspace.
      </p>
      <p>
Since both <m> V </m> and <m> W </m> are 2 dimensional vector spaces, they are isomorphic by <xref ref = "iso_same_dim" />. To exhibit an explicit isomorphism between the <m> V</m> and <m> W </m> we shall need find bases for both spaces.
      </p>

      <p>
        Since <m>V</m> is 2 dimensional, a basis for <m> V </m> consists of any two non-zero vectors in <m>V</m> that are not scalar multiples of one another. By inspection, we find the basis <m> \basis B_V = \bopen (1,0,1,1) , (0,1,-1,2) \bclose</m>. By similar reasoning, we find a basis <m> \basis B_W = \bopen  \frac{3}{8}x^2 - \frac{1}{2} , x - 1\bclose </m>. By <xref ref="defining_linear_map_on_basis" />, there is a unique linear map <m> T: V \to W </m> such that
        <md>
         <mrow> T((1,0,1,1)) \amp = \frac{3}{8}x^2 - \frac{1}{2} </mrow>

         <mrow> T((0,1,-1,2)) \amp = x -1 </mrow>
        </md>. This map is an isomorphism, as demonstrated by the proof of <xref ref ="iso_same_dim" />.
      </p>
    </solution>
  </exercise>

  <exercise>
    <statement>
      <p>
        Are the following vector spaces isomorphic?
        <me>
          V = \{ \ve{v} \in \mathbb{R}^3 : \ve{v} \times (1,2,3) = \ve{0} \}
        </me>
        <me>
          W = \left\{ M \in \Mat_{2,2} : M^T = -M \right\}
        </me>.
      </p>

      <p>
        If they are, construct an explicit isomorphism between them.
        If not, prove that they are not isomorphic.
      </p>
    </statement>
    <solution>
    <p>
      We use some geometry to find the dimension of <m> V</m>. <m> \ve v \in V  </m> if and only if
      <me>
|\ve v||(1,2,3)|\sin \theta =0 
    </me>
    where <m> \theta</m> is the angle between <m> \ve v </m> and <m> (1,2,3)</m>. Thus <m> V </m> consists of <m> \ve 0 </m> as well as all those vectors parallel to <m> (1,2,3)</m>. But this set is precisely all vectors of the form <m>k(1,2,3)</m> with <m> k \in \mathbb R </m>. Hence <m> V </m> is 1 dimensional with basis <m> \bopen (1,2,3) \bclose </m>.
    </p>
    <p>
<m> W </m> consists of all matrices <m>(a_{ij})</m> satisfying
<me>
\begin{bmatrix} a_{11} \mamp a_{21} \\ a_{12} \mamp a_{22}\end{bmatrix} = \begin{bmatrix} -a_{11} \mamp -a_{12} \\ -a_{21} \mamp -a_{22}\end{bmatrix}.
</me>
Thus <m> a_{11}  = a_{22} = 0 </m> and <m> b = -c</m>. So <m>W</m> consists of all those matrices  of the form
<me>
\begin{bmatrix} 0 \mamp k \\ -k \mamp 0\end{bmatrix}
</me>.
This also shows that 
<me>
\bopen \begin{bmatrix} 0 \mamp 1 \\ -1 \mamp 0\end{bmatrix} \bclose
</me>
is a basis for <m>W</m>. Hence <m> V </m> and <m> W</m> are isomorphic with the isomorphism given by the unique linear map <m> V \to W</m> satisfying
<me>
(1,2,3) \mapsto  \begin{bmatrix} 0 \mamp 1 \\ -1 \mamp 0\end{bmatrix}
</me>
    </p>
  </solution>
  </exercise>
  
</exercises>

<!-- <solutions divisional="solution answer" />  -->

</section>

