

<section xml:id="Ch3Sec2CompositionOfLinearMaps">
  <title>Composition of linear maps</title>
  <definition>
    <statement>
      <p>
        If <m>S : U \rightarrow V</m> and <m>T : V \rightarrow W</m> are linear maps,
        then the <term>composition of <m>T</m> with <m>S</m></term>
        is the map <m>T \circ S : U \rightarrow W</m> defined by
        <me>
          (T \circ S) (\ve{u}) := T(S(\ve{u}))
        </me>
        where <m>\ve{u}</m> is in <m>U</m>.
      </p>
    </statement>
  </definition>

  <p>
    See <xref ref="composition_of_linear_maps_fig">Figure</xref>.
  </p>

  <figure xml:id="composition_of_linear_maps_fig">
    <caption>Composition of linear maps.</caption>
    <image>

<latex-image>
          <![CDATA[\begin{tikzpicture}[xscale=1.2]
    \draw (0, 0) circle (1);
    \draw (-4,0) circle (1);
    \draw (-8,0) circle (1);
    \node at (0, -1.3) {\(U\)};
    \node at (-4, -1.3) {\(V\)};
    \node at (-8, -1.3) {\(W\)};
    \draw[->] (-1.2, 0.3) to[out=150, in=30] node[above] {\(S\)} (-2.8, 0.3);
    \draw[->] (-5.2, 0.3) to[out=150, in=30] node[above] {\(T\)} (-6.8, 0.3);
    \draw[->] (-1.2, 0.6) to[out=140, in=40] node[above] {\(T\circ S\)} (-7, 0.6);
    \node (u) at (0, -0.5) {\(\ve{u}\)};
    \node (v) at (-4, -0.5) {\(S(\ve{u})\)};
    \node (w) at (-8, -0.5) {\(T(S(\ve{u}))\)};
    \draw[|->] (u) to[out=170, in=10] (v);
    \draw[|->] (v) to[out=170, in=10] (w);\end{tikzpicture}]]>
</latex-image>
    </image>

  </figure>

  <assemblage>
    <p>
      The standard convention in mathematics is to write the evaluation of a function from right-to-left, eg.
      <m>f(x)</m>.
      That is, you start with the right hand symbol <m>x</m>,
      then you apply <m>f</m>.
      So the most natural way to draw these pictures is from right-to-left!
    </p>
  </assemblage>

  <example>
    <statement>
      <p>
        Let <m>S : \mathbb{R}^3 \rightarrow \Poly_2</m> and
        <m>T : \Poly_2 \rightarrow \Poly_4</m> be the linear maps defined by
        <me>
          S( (a,b,c) ) := ax^2 + (a-b)x + c,  T(p(x)) = x^2 p(x)
        </me>
      </p>

      <p>
        Then <m>T\circ S</m> can be computed as follows:
        <md>
          <mrow>(T \circ S)((a,b,c)) \amp = T(S((a,b,c)))</mrow>
          <mrow>\amp = T(ax^2 + (a-b)x + c)</mrow>
          <mrow>\amp = x^2 (ax^2 + (a-b)x + c)</mrow>
          <mrow>\amp = ax^4 + (a-b)x^3 + cx^2</mrow>
        </md>.
      </p>
    </statement>
  </example>

  <proposition>
    <statement>
      <p>
        If <m>S : U \rightarrow V</m> and <m>T : V \rightarrow W</m> are linear maps,
        then <m>T \circ S : U \rightarrow W</m> is also a linear map.
      </p>
    </statement>
  </proposition>

  <proof>
    <p>
      Let <m>\ve{u_1}, \ve{u}_2 \in U</m>.
      Then:
      <md>
        <mrow>(T \circ S) (\ve{u}_1 + \ve{u}_2)   \amp = T(S(\ve{u}_1 + \ve{u}_2)) \amp  \mbox{(defn of \(T \circ S\))}</mrow>
        <mrow>\amp = T(S(\ve{u}_1) + S(\ve{u}_2)) \amp  \mbox{ (\(S\) is linear)}</mrow>
        <mrow>\amp = T(S(\ve{u}_1)) + T(S(\ve{u}_2)) \amp  \mbox{ (\(T\) is linear)}</mrow>
        <mrow>\amp = (T \circ S) (\ve{u}_1) + (T \circ S)(\ve{u}_2) \amp  \mbox{(defn of \(T \circ S\))}</mrow>
      </md>
    </p>

    <p>
      Similarly,
      <md>
        <mrow>(T \circ S) (k \ve{u}) \amp = T(S(k \ve{u})) \amp  \mbox{(defn of \(T \circ S\))}</mrow>
        <mrow>\amp = T(kS(\ve{u})) \amp  \mbox{(\(S\) is linear)}</mrow>
        <mrow>\amp = k T(S(\ve{u})) \amp  \mbox{(\(T\) is linear)}</mrow>
        <mrow>\amp = k (T \circ S) (\ve{u}) \amp  \mbox{(defn of \(T \circ S\))}</mrow>
      </md>
    </p>
  </proof>

  <example>
    <statement>
    <p>
      Consider the antiderivative (<m>A</m>) and derivative (<m>D</m>) linear maps
      <md>
        <mrow>A : \Poly_n \amp  \rightarrow \Poly_{n+1}</mrow>
        <mrow>D : \Poly_{n+1} \amp  \rightarrow \Poly_n</mrow>
      </md>.
    </p>

    <p>
      Is <m>D \circ A = \id_{\Poly_n}</m>?
    </p>
    <solution>
      <p>
        We compute the action of <m>D \circ A</m> on the basis <m>x^k</m>,
        <m>k=0 \ldots n</m> of <m>\Poly_n</m>:
        <me>
          x^k \stackrel{A}{\mapsto} \frac{x^{k+1}}{k+1} \stackrel{D}{\mapsto} \frac{k+1}{k+1} x^k = x^k
        </me>
      </p>

      <p>
        Hence for <m>k=0 \ldots n</m>,
        <md>
          <mrow>(D \circ A) (x^k) \amp = x^k</mrow>
          <mrow>\amp = \id_{\Poly_n} (x^k)</mrow>
        </md>.
      </p>

      <p>
        Since <m>D \circ A</m> and
        <m>\id_{\Poly_n}</m> agree on a basis for <m>\Poly_n</m>,
        they agree on all vectors <m>\ve{p} \in \Poly_n</m> by <xref ref="defining_linear_map_on_basis">Proposition</xref>.
        Hence <m>D \circ A = \id_{\Poly_n}</m>.
      </p>

      <assemblage>
        <p>
          In fact, the statement that
          <m>D \circ A = \id_{\Poly_n}</m> is precisely Part I of the Fundamental Theorem of Calculus,
          applied to the special case of polynomials!
        </p>
      </assemblage>

    </solution>


    </statement>
  </example>

      <exercise>
      <statement>
        <p>
          Is <m>A \circ D = \id_{\Poly_{n+1}}</m>?
          If it is, prove it.
          If it is not, give an explicit counterexample.
        </p>
      </statement>

      <solution>
        <p>
The statement is not true! For example, let <m> \ve p(x) = x + 1 </m>.
Then
<me>
(A \circ D)(x + 1)  = A(1) = x \neq x + 1.
</me>
</p>
      </solution>
    </exercise>


  <exercises>
  <exercise>
    <statement>
      <p>
        Let <m>R_\theta : \mathbb{R}^2 \rightarrow \mathbb{R}^2</m> be the <sq>rotation by <m>\theta</m></sq> map from <xref ref="rotation-map-example-complete">Example</xref>,
        <me>
          R( (x,y)) = (x \cos \theta - y \sin \theta, \, x \sin \theta + y \cos \theta)
        </me>.
      </p>

      <p>
        Check algebraically that <m>R_\phi \circ R_\theta = R_{\phi + \theta}</m> by computing the action of the linear maps on both sides of this equation on an arbitrary vector <m>(x,y) \in \mathbb{R}^2</m>.
      </p>
    </statement>
    <solution>
      <p>
        <md>
        <mrow>R_\phi R_\theta (x,y) \amp = R_\phi (x\cos\theta - y\sin\theta, x\sin\theta + y\cos\theta)</mrow>
        <mrow>\amp =  \left((x\cos\theta-y\sin\theta)\cos\phi - (x\sin\theta + y \cos\theta)\sin\phi ,\, (x\cos\theta - y\sin\theta)\sin\phi + (x\sin\theta + y\cos\theta)\cos \phi\right) </mrow>
        <mrow> \amp = \left(x(\cos\theta\cos\phi - \sin\theta\sin\phi) - y(\sin\theta\cos\phi + \cos\theta\sin\phi),\, x(\cos\theta\sin\phi + \sin\theta\cos\phi) + y(\cos\theta\cos\phi - \sin\theta\sin\phi)\right) </mrow>
        <mrow> \amp = \left(x\cos(\theta + \phi) - y\sin(\theta + \phi), \,x\sin(\theta+\phi) + y\cos(\theta + \phi_)\right) </mrow>
        <mrow> \amp = R_{\phi + \theta}(x,y) </mrow>
      </md>
</p>
    </solution>
  </exercise>

  <exercise>
    <statement>
      <p>
        Let <m>M : \Poly_3 \rightarrow \Poly_4</m> be the <sq>multiplication by <m>x</m></sq> map,
        <m>M(p)(x) = x p(x)</m>.
        Let <m>S : \Poly_4 \rightarrow \Poly_4</m> be the map <m>S(p(x)) = p(x-1)</m>.
        Similarly let <m>T : \Poly_3 \rightarrow \Poly_3</m> be the map <m>T(p(x)) = p(x-1)</m>.
        Compute <m>S \circ M</m> and <m>M \circ T</m>.
        Are they equal?
      </p>
    </statement>
    <solution>
      <p>
        <me>
        (S \circ M)(p(x)) = S(M(p(x))) = S(x p(x)) = (x-1)p(x-1)
      </me>
      whereas
      <me>
      (M \circ S)(p(x)) = M(p(x-1)) = xp(x-1).
    </me>
Thus <m> S \circ M \neq M \circ S </m>.
      </p>
    </solution>
  </exercise>
  </exercises>

 <!-- <solutions divisional="solution answer" />  -->


</section>

