<section xml:id="Tut4">
<title>W214 2019, Linear Algebra Tutorial 4</title>
<shorttitle>Tutorial 4</shorttitle>

<p>Note: You are welcome to use the <url href="https://sagecell.sagemath.org/">SageMath cell server</url> to help you solve some of the problems below, or at least to check your calculations. </p>

<exercises>

<assemblage><title>2.4 Coordinate vectors</title>
</assemblage>

  <exercise xml:id="matrix_basis_exercise-tut">
    <statement>
      <p>
        Let <m>\basis{B} = \bopen \mat{B}_1, \mat{B}_2, \mat{B}_3, \mat{B}_4 \bclose </m> be the basis of <m>\Mat_{2,2}</m> given by
        <me>
 \mat{B}_1 = \begin{bmatrix}
1 &amp; 0 \\
0 &amp; 1
\end{bmatrix}, \mat{B}_2 =
 \begin{bmatrix}
1 &amp; 0\\
0&amp; -1
\end{bmatrix},
 \mat{B}_3 = \begin{bmatrix}
1 &amp; 1\\
1 &amp; 1
\end{bmatrix},
 \mat{B}_4 = \begin{bmatrix}
0 &amp; 1\\
-1 &amp; 0
\end{bmatrix}
 </me>.
      </p>

      <p>
        Determine <m>[\mat{A}]_\basis{B}</m>, where
        <me>
          \mat{A} =  \begin{bmatrix}
1 &amp; 2\\
3 &amp; 4
\end{bmatrix}.
        </me>
      </p>
    </statement>
    <solution>
      <p>
To determine  <m>[\mat{A}]_\basis{B}</m>, we must find the scalars <m>a_1 , a_2 , a_3, a_4 </m> satisfying
<me>
a_1 \mat{B_1} + a_2\mat{B_2} + a_3\mat{B_3} + a_4\mat{B_4} = \mat A.
</me>
This results in a system of 4 linear equations in 4 variables, one equation for each entry in <m>\mat A </m>:
<md>
<mrow>a_1 + a_2 + a_3 = 1 </mrow>
<mrow> a_3 + a_4 = 2 </mrow>
<mrow> a_3 - a_4 = 3 </mrow>
<mrow> a_1 - a_2 + a_3 = 4</mrow>
</md>
Solving this equation, we get
<me>
a_1  = 0, \quad
a_2  = -\frac{3}{2}, \quad
a_3  = \frac{5}{2}, \quad
a_4  = -\frac{1}{2}.
</me>
Hence <me>
[\mat{A}]_\basis{B} = \begin{bmatrix} 0 \\ -\frac{3}{2} \\ \frac{5}{2} \\ -\frac{1}{2} \end{bmatrix}
</me>
      </p>
    </solution>
  </exercise>

  <exercise>
    <statement>
        <ol>
          <li>
            <title>(a)</title>
            <p>Find a basis <m>\basis{B}</m> for the vector space
        <me>
          V := \{ p \in \Poly_2 : p(2) = 0 \}
        </me>.
      </p>
          </li>
          <li>
            <title>(b)</title>
            <p>
               Consider <m>p(x) = x^2 + x - 6</m>. Show that <m>p \in V</m>.
            </p>
          </li>

          <li>
            <title>(c)</title>
            <p>
              Determine the coordinate vector of <m>p</m> with respect to your basis <m>\basis{B}</m>,
              i.e. determine <m>[p]_\basis{B}</m>.
            </p>
          </li>
        </ol>
    </statement>
  </exercise>

<exercise>
  <statement> <p>Consider the vector space <m>W</m> from <xref ref="dimension_of_hyperplane"/>,
  <me>
  W = \{ (w_1, w_2, w_3) \in \mathbb{R}^3 : w_1 + 2w_2 + 3w_3 = 0 \},
</me>
and the following bases for <m>W</m>:
<me>
 \basis{B} = \bopen \ve{a}, \ve{b} \bclose, \quad  \basis{C} = \bopen \ve{u}, \ve{v} \bclose
</me>
where
<md>
 <mrow> \ve{a} \amp = (1, 0, -\frac{1}{3}), \amp \ve{b} \amp = (0, 1, - \frac{2}{3}) </mrow>
 <mrow> \ve{u} \amp = (1, 2, -\frac{5}{3}), \amp \ve{v} \amp = (-4, 2, 0) </mrow>
</md>
Consider the vector <m>\ve{w} = (-2, 4, -2) \in \mathbb{R}^3</m>. 
 <ol>
  <li>Show that <m>\ve{w} \in W</m>. </li>
  <li>Determine <m>[\ve{w}]_{\basis{B}}</m>.</li>
  <li>Determine <m>[\ve{w}]_{\basis{C}}</m>. </li>
 </ol>
</p>
</statement>
</exercise>

    <exercise>
    <statement>
      <p>Let <m>V</m> be the vector space of solutions to the differential equation
      <men xml:id="diff_eqn_exerc_1_tut">
        y^{''} + y = 0.
      </men>
      </p>
      <ol>
        <li> <p> Show that <m>\basis{B} = \bopen \cos x, \, \sin x \bclose </m> is a basis for <m>V</m>. </p> </li>
        <li> <p> Let <m>y \in V</m> be defined as the unique solution to the differential equation in <xref ref="diff_eqn_exerc_1_tut"/> satisfying
        <me>
        y(\frac{\pi}{6}) = 1, \quad y'(\frac{\pi}{6}) = 0.
      </me>
      (Note that we can indeed define <m>y</m> uniquely in this way due to <xref ref="diff_eqn_exist_unique"/>.) Compute <m>[y]_\basis{B}</m>. </p>
    </li>
    <li> <p>Let <m>z(x) = \cos\left(x - \frac{\pi}{3} \right)</m>.</p>
      <ol>
        <li>Show that <m>z \in V</m> by checking that it solves the differential equation <xref ref="diff_eqn_exerc_1_tut"/>.</li>
        <li>Determine <m>[z]_{\basis{B}}</m>. </li>

      </ol>

    </li>
      </ol>
    </statement>
    </exercise>

<assemblage><title>2.5 Change of basis</title>
</assemblage>



<exercise>
    <statement>
      <p>
        This is a continuation of <xref ref="matrix_basis_exercise-tut">Exercise</xref>.
        Consider the following two bases for <m>\Mat_{2,2}</m>:
        <me>
\basis B = \left\{ 
\text{B}_1 =   \begin{bmatrix} 1 &amp;  0 \\ 0 &amp;  1 \end{bmatrix}, \,
\text{B}_2 =   \begin{bmatrix} 1 &amp;  0\\ 0 &amp;  -1 \end{bmatrix}, \, 
\text{B}_3 =   \begin{bmatrix} 1 &amp;  1 \\ 1 &amp;  1 \end{bmatrix}, \,
\text{B}_4 =   \begin{bmatrix} 0 &amp;  1 \\ -1 &amp; 0 \end{bmatrix}               
\right\}
      </me>

      <me>
\basis C = \left\{ 
\text{C}_1 =   \begin{bmatrix} 1 &amp;  1 \\ 0 &amp;  0  \end{bmatrix}, \,
\text{C}_2 =   \begin{bmatrix} 1 &amp;  -1 \\ 0 &amp;  0 \end{bmatrix}, \, 
\text{C}_3 =   \begin{bmatrix} 0 &amp;  0 \\ 1 &amp;  1 \end{bmatrix}, \,
\text{C}_4 =   \begin{bmatrix} 0 &amp;  0 \\ 1 &amp; -1 \end{bmatrix}               
\right\}
      </me>

        <dl>
          <li>
            <title>(a)</title>
            <p>
              Determine the change-of-basis matrices
              <m>\mat{P}_{\basis{C} \leftarrow \basis{B}}</m> and <m>\mat{P}_{\basis{B} \leftarrow \basis{C}}</m>.
            </p>
          </li>

          <li>
            <title>(b)</title>
            <p>
              Determine <m>[\mat{A}]_\basis{B}</m> and <m>[\mat{A}]_\basis{C}</m> where
              <me>
                A = \begin{bmatrix} 1 &amp; 2 \\ 3 &amp; 4 \end{bmatrix}
              </me>.
            </p>
          </li>

          <li>
            <title>(c)</title>
            <p>
              Check that <m>[\mat{A}]_\basis{C} = \mat{P}_{\basis{C} \leftarrow \basis{B}} [\mat{A}]_\basis{B}</m> and that <m>[\mat{A}]_\basis{B} = \mat{P}_{\basis{B} \leftarrow \basis{C}} [\mat{A}]_\basis{C}</m>.
            </p>
          </li>
        </dl>
      </p>
    </statement>
  </exercise>


  <exercise>
    <statement><p><xref ref="w_in_b_basis_tut"/> displays a basis <m>\basis{B} = \bopen \ve{b}_1, \ve{b}_2 \bclose</m> for <m>\mathbb{R}^2</m>, a background of integral linear combinations of <m>\ve{b}_1</m> and <m>\ve{b}_2</m>, and a certain vector <m>\ve{w} \in \mathbb{R}^2</m>. Similarly, <xref ref="w_in_c_basis_tut"/> displays another basis <m>\basis{C} = \bopen \ve{c}_1, \ve{c}_2 \bclose</m> for <m>\mathbb{R}^2</m>, a background of integral linear combinations of <m>\ve{c}_1</m> and <m>\ve{c}_2</m>, and the same vector <m>\ve{w} \in \mathbb{R}^2</m>. </p>
    <sidebyside>
      <figure xml:id="w_in_b_basis_tut">
      <caption>The vector <m>\ve{w}</m> against a background of integral linear combinations of the basis vectors from <m>\basis{B}</m>. </caption>
      <image>

<latex-image>
          <![CDATA[\begin{tikzpicture}[scale=0.5]
  \draw[red, dotted] (-3, -9) -- (9, -3);
  \draw[red, dotted] (-4, -7) -- (8, -1);  
  \draw[red, dotted] (-5, -5) -- (7, 1);
  \draw[red, dotted] (-6, -3) -- (6, 3);
  \draw[red, dotted] (-7, -1) -- (5, 5);
  \draw[red, dotted] (-8, 1) -- (4, 7);
  \draw[red, dotted] (-9, 3) -- (3, 9);

  \draw[red, dotted] (-3, -9) -- (-9, 3);
  \draw[red, dotted] (-1, -8) -- (-7, 4);
  \draw[red, dotted] (1, -7) -- (-5, 5);
  \draw[red, dotted] (3, -6) -- (-3, 6);
  \draw[red, dotted] (5, -5) -- (-1, 7);
  \draw[red, dotted] (7, -4) -- (1, 8);
  \draw[red, dotted] (9, -3) -- (3, 9);

  \draw[very thick, red, ->] (0,0) -- node[pos=1.3] {\(\ve{b}_1\)} (2,1); 
  \draw[very thick, red, ->] (0,0) -- node[pos=1.3] {\(\ve{b}_2\)} (-1,2);
  \draw[thick, ->] (0,0) -- node[pos=1.2] {\(\ve{w}\)} (3,-1);\end{tikzpicture}]]>
</latex-image>
      </image>
    </figure>

  <figure xml:id="w_in_c_basis_tut">
    <caption>The vector <m>\ve{w}</m> against a background of integral linear combinations of the basis vectors from <m>\basis{C}</m>. </caption>
      <image>

<latex-image>
          <![CDATA[\begin{tikzpicture}[scale=0.5]
  \draw[blue, dotted] (0, -6) -- (6, 0);
  \draw[blue, dotted] (-1, -5) -- (5, 1);
  \draw[blue, dotted] (-2, -4) -- (4, 2);
  \draw[blue, dotted] (-3, -3) -- (3, 3);
  \draw[blue, dotted] (-4, -2) -- (2, 4);
  \draw[blue, dotted] (-5, -1) -- (1, 5);
  \draw[blue, dotted] (-6, 0) -- (0, 6);

  \draw[blue, dotted] (0, -6) -- (-6, 0);
  \draw[blue, dotted] (1, -5) -- (-5, 1);
  \draw[blue, dotted] (2, -4) -- (-4, 2);
  \draw[blue, dotted] (3, -3) -- (-3, 3);
  \draw[blue, dotted] (4, -2) -- (-2, 4);
  \draw[blue, dotted] (5, -1) -- (-1, 5);
  \draw[blue, dotted] (6, 0) -- (0, 6);

  \draw[very thick, blue, ->] (0,0) -- node[pos=1.6] {\(\ve{c}_1\)} (1,1); 
  \draw[very thick, blue, ->] (0,0) -- node[pos=1.6] {\(\ve{c}_2\)} (-1,1);
  \draw[thick, ->] (0,0) -- node[pos=1.2] {\(\ve{w}\)} (3,-1);\end{tikzpicture}]]>
</latex-image>
      </image>

    </figure>
  </sidebyside>
    <ol>
      <li xml:id="ch-basis-exercise2-tut">
        <p> Determine <m>[\ve{w}]_\basis{B}</m>, directly from <xref ref="w_in_b_basis_exc"/>. </p>
      </li>
      <li xml:id="ch-basis-exercise3-tut">
        <p> Determine <m>[\ve{w}]_\basis{C}</m>, directly from <xref ref="w_in_c_basis_exc"/>. </p>
      </li>
      <li xml:id="ch-basis-exercise1-tut"> <p>The following figure displays the <m>\basis{B}</m> basis against a background of integral linear combinations of the <m>\basis{C}</m> basis:

    <sidebyside>
    <image width="60%">

<latex-image>
          <![CDATA[\begin{tikzpicture}[scale=0.5]

  \draw[blue, dotted] (0, -6) -- (6, 0);
  \draw[blue, dotted] (-1, -5) -- (5, 1);
  \draw[blue, dotted] (-2, -4) -- (4, 2);
  \draw[blue, dotted] (-3, -3) -- (3, 3);
  \draw[blue, dotted] (-4, -2) -- (2, 4);
  \draw[blue, dotted] (-5, -1) -- (1, 5);
  \draw[blue, dotted] (-6, 0) -- (0, 6);

  \draw[blue, dotted] (0, -6) -- (-6, 0);
  \draw[blue, dotted] (1, -5) -- (-5, 1);
  \draw[blue, dotted] (2, -4) -- (-4, 2);
  \draw[blue, dotted] (3, -3) -- (-3, 3);
  \draw[blue, dotted] (4, -2) -- (-2, 4);
  \draw[blue, dotted] (5, -1) -- (-1, 5);
  \draw[blue, dotted] (6, 0) -- (0, 6);

  \draw[very thick, blue, ->] (0,0) -- node[pos=1.6] {\(\ve{c}_1\)} (1,1); 
  \draw[very thick, blue, ->] (0,0) -- node[pos=1.6] {\(\ve{c}_2\)} (-1,1);
  \draw[very thick, red, ->] (0,0) -- node[pos=1.3] {\(\ve{b}_1\)} (2,1); 
  \draw[very thick, red, ->] (0,0) -- node[pos=1.3] {\(\ve{b}_2\)} (-1,2);\end{tikzpicture}]]>
</latex-image>
    </image>
  </sidebyside>
        Determine the change-of-basis matrix <m>\mat{P}_{\basis{C} \leftarrow \basis{B}}</m>. (You may assume that all coefficients are either integers and half-integers.)</p>
      </li>
      <li> Multiply the matrix you computed in <xref ref="ch-basis-exercise1-tut" text="title">(c)</xref> with the column vector you computed in <xref ref="ch-basis-exercise2-tut" text="title">(a)</xref>. That is, compute the product <m>\mat{P}_{\basis{C} \leftarrow \basis{B}} [\mat{w}]_{\basis{B}}</m>. Is your answer the same as what you obtained in <xref ref="ch-basis-exercise3-tut" text="title">(b)</xref>?
    </li>
    </ol>
    </statement>
  </exercise>

<exercise>
  <statement>
    Consider the following three bases for <m>\mathbb R^3</m>:
    <md>
    <mrow>  \mathcal A = \bopen (1,0,0), (0,1,0), (0,0,1) \bclose </mrow>
      <mrow> \mathcal B = \bopen (2,1,1) , (1,1,1), (0,2,1) \bclose </mrow>
     <mrow> \mathcal C= \bopen (1,2,3),(0,1,0),(1,0,1) \bclose</mrow>.
    </md>
    Compute <m>\mat{P}_{\basis{C} \leftarrow \basis{B}}, \mat{P}_{\basis{B} \leftarrow \basis{A}}, \mat{P}_{\basis{C} \leftarrow \basis{A}}</m> and verify the equation
    <me>
\mat{P}_{\basis{C} \leftarrow \basis{B}}  \mat{P}_{\basis{B} \leftarrow \basis{A}} =  \mat{P}_{\basis{C} \leftarrow \basis{A}}.
  </me>
  </statement>
</exercise>


</exercises>

</section>


